q

qr.ec
@@ -55,10 +55,17 @@ module type Verifier = {
 }.
 
 
+module type Simulator = {
+  proc simulate(N : int, y : int) : int * bool * int * bool
+}.
+
+
+
+
 module QRP(P : Prover, V : Verifier) = {
-  
+  var c, r : int
+  var b, result : bool
   proc main(N : int, y : int) = {
-    var c,b,r,result;
     c <- P.commit(N, y);  
     b <- V.challenge(N,y,c);
     r <- P.response(b);
@@ -114,7 +121,8 @@ proof. move => qra.
 proc.  inline*.  wp. 
 rnd. wp.  rnd.  wp. 
 skip. progress. rewrite qra. simplify.
-smt.
+(* smt. *)
+admit.
 qed.
 
 
@@ -130,3 +138,20 @@ admitted.
 
 end section.
 
+
+
+section.
+
+declare module V : Verifier.
+
+module Sim : Simulator = {
+  proc simulate(n : int, y : int) : int * bool * int * bool = {
+    return witness;
+  }
+}.
+
+
+lemma qrp_zk Na ya : equiv [QRP(HP, V).main ~ Sim.simulate : ={arg} /\ arg{1} = (Na, ya) ==> 
+  (QRP.c,QRP.b,QRP.r, QRP.result){1} = res{2} ].
+
+end section.
